bigg reorganization

theories/terms.v
@@ -1,8 +1,8 @@
 (* Bunched terms *)
 From Coq Require Import ssreflect.
 From bunched.algebra Require Import bi.
-From bunched Require Import syntax interp.
-From stdpp Require Import prelude base gmap fin_sets functions mapset.
+From bunched Require Import syntax interp prelude.sets.
+From stdpp Require Import prelude base gmap functions.
 
 (** * Bunched terms *)
 Inductive bterm (var : Type) : Type :=
@@ -17,7 +17,6 @@ Arguments TSemic {_} T1 T2.
 Global Instance bterm_eqdecision `{EqDecision A} : EqDecision (bterm A).
 Proof. solve_decision. Qed.
 Global Instance bterm_countable : Countable (bterm nat).
-Proof.
 Proof.
  set (enc :=
    fix go T :=
@@ -38,6 +37,22 @@ Proof.
  induction x; simpl; eauto; by rewrite IHx1 IHx2.
 Defined.
 
+Fixpoint bterm_alg_act {PROP : bi} `{!EqDecision V,!Countable V}
+         (T : bterm V) (Xs : V → PROP) : PROP :=
+  match T with
+  | Var v => Xs v
+  | TComma T1 T2 => bterm_alg_act T1 Xs ∗ bterm_alg_act T2 Xs
+  | TSemic T1 T2 => bterm_alg_act T1 Xs ∧ bterm_alg_act T2 Xs
+  end%I.
+
+Fixpoint bterm_ctx_act `{!EqDecision V,!Countable V}
+         (T : bterm V) (Δs : V → bunch) : bunch :=
+  match T with
+  | Var v => Δs v
+  | TComma T1 T2 => bterm_ctx_act T1 Δs,, bterm_ctx_act T2 Δs
+  | TSemic T1 T2 => bterm_ctx_act T1 Δs;, bterm_ctx_act T2 Δs
+  end%B.
+
 Global Instance bterm_fmap : FMap bterm :=
   fix go _ _ f T { struct T } := let _ : FMap _ := go in
   match T with
@@ -53,8 +68,7 @@ Fixpoint term_fv `{!EqDecision V,!Countable V} (T : bterm V) : gset V :=
   | TSemic T1 T2 => term_fv T1 ∪ term_fv T2
   end.
 
-Fixpoint linear_bterm `{!EqDecision V,!Countable V}
-  (T : bterm V) : Prop :=
+Fixpoint linear_bterm `{!EqDecision V,!Countable V} (T : bterm V) : Prop :=
   match T with
   | Var x => True
   | TComma T1 T2
@@ -63,6 +77,8 @@ Fixpoint linear_bterm `{!EqDecision V,!Countable V}
     linear_bterm T1 ∧ linear_bterm T2
   end.
 
+
+(** ** Term linearization *)
 (** We define a "linearization" of a term:
     for a example a term
       (X₁;X₁),X₂
@@ -71,7 +87,7 @@ Fixpoint linear_bterm `{!EqDecision V,!Countable V}
     with an associated renaming
       { Y₁ => X₁, Y₂ => X₁, Y₃ => X₂ }
    *)
-Local Fixpoint linearize_pre (T : bterm nat) (idx : nat) : nat * gmap nat nat * bterm nat :=
+Fixpoint linearize_pre (T : bterm nat) (idx : nat) : nat * gmap nat nat * bterm nat :=
   match T with
   | Var x => (idx + 1, {[ idx := x ]}, Var idx)
   | TComma T1 T2 =>
@@ -87,27 +103,35 @@ Local Fixpoint linearize_pre (T : bterm nat) (idx : nat) : nat * gmap nat nat * 
 Definition linearize_bterm (T : bterm nat) : bterm nat := snd (linearize_pre T 0).
 Definition linearize_bterm_ren (T : bterm nat) : gmap nat nat := snd $ fst (linearize_pre T 0).
 
-
-(** ** Actions on bunches and and interpretation in BI algebras *)
-Fixpoint bterm_ctx_act `{!EqDecision V,!Countable V}
-         (T : bterm V) (Δs : V → bunch) : bunch :=
+(** ** Term "folding" *)
+Fixpoint bterm_gset_fold (T : bterm (gset nat)) : gset (bterm nat) :=
   match T with
-  | Var v => Δs v
-  | TComma T1 T2 => bterm_ctx_act T1 Δs,, bterm_ctx_act T2 Δs
-  | TSemic T1 T2 => bterm_ctx_act T1 Δs;, bterm_ctx_act T2 Δs
-  end%B.
+  | Var X => set_map Var X
+  | TComma T1 T2 =>
+      let S1 := bterm_gset_fold T1 in
+      let S2 := bterm_gset_fold T2 in
+      set_map_2 TComma S1 S2
+  | TSemic T1 T2 =>
+      let S1 := bterm_gset_fold T1 in
+      let S2 := bterm_gset_fold T2 in
+      set_map_2 TSemic S1 S2
+  end.
 
-Fixpoint bterm_alg_act {PROP : bi} `{!EqDecision V,!Countable V}
-         (T : bterm V) (Xs : V → PROP) : PROP :=
-  match T with
-  | Var v => Xs v
-  | TComma T1 T2 => bterm_alg_act T1 Xs ∗ bterm_alg_act T2 Xs
-  | TSemic T1 T2 => bterm_alg_act T1 Xs ∧ bterm_alg_act T2 Xs
-  end%I.
+Definition bterm_gset_fmap (f : nat → nat) (T : bterm (gset nat)) : bterm (gset nat) := set_map f <$> T.
+
+(** ** Structural rules *)
+
+Definition structural_rule := (list (bterm nat) * bterm nat)%type.
+Definition is_analytical (s : structural_rule) := linear_bterm (snd s).
+Definition rule_valid (s : structural_rule) (PROP : bi) : Prop :=
+  ∀ (Xs : nat → PROP),
+    bterm_alg_act (snd s) Xs ⊢
+       ∃ Ti' : {Ti : bterm nat | Ti ∈ fst s }, bterm_alg_act (proj1_sig Ti') Xs.
+
 
 (** * Properties *)
 
-(** On modifications/operations: *)
+(** ** fmap properties *)
 Lemma bterm_fmap_ext {A B} `{EqDecision A, Countable A} (f g : A → B) (t1 t2 : bterm A) :
   (∀ x, x ∈ term_fv t1 → f x = g x) → t1 = t2 → fmap f t1 = fmap g t2.
 Proof.
@@ -129,6 +153,130 @@ Proof.
   - rewrite IHT1 IHT2 //.
 Qed.
 
+(** ** interpretation properties *)
+Lemma bterm_ctx_act_fv `{!EqDecision V,!Countable V} (T : bterm V) Δs Γs :
+  (∀ i : V, i ∈ term_fv T → Δs i = Γs i) →
+  bterm_ctx_act T Δs = bterm_ctx_act T Γs.
+Proof.
+  induction T; simpl.
+  - set_solver.
+  - set_unfold. intros H.
+    rewrite IHT1; eauto. rewrite IHT2; eauto.
+  - set_unfold. intros H.
+    rewrite IHT1; eauto. rewrite IHT2; eauto.
+Qed.
+Lemma bterm_alg_act_fv `{!EqDecision V,!Countable V} {PROP : bi}
+      (T : bterm V) Δs Γs :
+  (∀ i : V, i ∈ term_fv T → Δs i ≡ Γs i) →
+  bterm_alg_act T Δs ≡ bterm_alg_act (PROP:=PROP) T Γs.
+Proof.
+  induction T; simpl.
+  - set_solver.
+  - set_unfold. intros H.
+    rewrite IHT1; eauto. rewrite IHT2; eauto.
+  - set_unfold. intros H.
+    rewrite IHT1; eauto. rewrite IHT2; eauto.
+Qed.
+
+Lemma bterm_alg_act_mono {PROP : bi} `{!EqDecision V, !Countable V}
+      (T : bterm V) Xs Ys :
+  (∀ i, Xs i ⊢ Ys i) →
+  bterm_alg_act T Xs ⊢ bterm_alg_act (PROP:=PROP) T Ys.
+Proof.
+  intros HXY. induction T; simpl; auto.
+  all: by rewrite IHT1 IHT2.
+Qed.
+
+Lemma bterm_alg_act_mono' {PROP : bi} `{!EqDecision V, !Countable V}
+      (T : bterm V) Xs Ys :
+  (∀ i, i ∈ term_fv T → Xs i ⊢ Ys i) →
+  bterm_alg_act T Xs ⊢ bterm_alg_act (PROP:=PROP) T Ys.
+Proof.
+  intros HXY. induction T; simpl; eauto.
+  - apply HXY. set_solver.
+  - f_equiv.
+    + apply IHT1. set_solver.
+    + apply IHT2. set_solver.
+  - f_equiv.
+    + apply IHT1. set_solver.
+    + apply IHT2. set_solver.
+Qed.
+
+(** Interpretation of bunches is a homomorphism w.r.t. bunched terms:
+<<
+  ⟦ T(Δs) ⟧ = ⟦ T ⟧ (⟦ Δs ⟧)
+>>
+*)
+Lemma bterm_ctx_alg_act {PROP : bi} `{!EqDecision V,!Countable V}
+      (T : bterm V) (Δs : V → bunch) (s : atom → PROP) :
+  bunch_interp s (bterm_ctx_act T Δs) =
+  bterm_alg_act T (bunch_interp s ∘ Δs).
+Proof.
+  induction T; simpl.
+  - reflexivity.
+  - by rewrite IHT1 IHT2.
+  - by rewrite IHT1 IHT2.
+Qed.
+
+(** Linear bunched terms can be viewed as _bunches with holes_, when
+restricted to one free variable. *)
+Lemma blinterm_ctx_act_insert `{!EqDecision V, !Countable V} (T : bterm V) Δs i :
+  linear_bterm T →
+  i ∈ term_fv T →
+  ∃ (Π : bunch_ctx), ∀ Γ , fill Π Γ = bterm_ctx_act T (<[i:=Γ]>Δs).
+Proof.
+  revert i. induction T=>i; simpl ; intros Hlin Hi.
+  - exists []. intros Γ. assert ( i = x) as -> by set_solver.
+    by rewrite functions.fn_lookup_insert.
+  - destruct Hlin as (Hdisj & Hlin1 & Hlin2).
+    set_unfold.
+    destruct Hi as [Hi1 | Hi2].
+    + destruct (IHT1 i Hlin1 Hi1) as (Π₁ & HΠ1).
+      exists (Π₁++[CtxCommaL (bterm_ctx_act T2 Δs)]).
+      intros Γ. rewrite fill_app /=.
+      rewrite HΠ1. f_equiv.
+      assert (i ∉ term_fv T2).
+      { set_solver. }
+      apply bterm_ctx_act_fv.
+      intros j. destruct (decide (i = j)) as [->|?].
+      { naive_solver. }
+      rewrite functions.fn_lookup_insert_ne//.
+    + destruct (IHT2 i Hlin2 Hi2) as (Π₁ & HΠ1).
+      exists (Π₁++[CtxCommaR (bterm_ctx_act T1 Δs)]).
+      intros Γ. rewrite fill_app /=.
+      rewrite HΠ1. f_equiv.
+      assert (i ∉ term_fv T1).
+      { set_solver. }
+      apply bterm_ctx_act_fv.
+      intros j. destruct (decide (i = j)) as [->|?].
+      { naive_solver. }
+      rewrite functions.fn_lookup_insert_ne//.
+  - destruct Hlin as (Hdisj & Hlin1 & Hlin2).
+    set_unfold.
+    destruct Hi as [Hi1 | Hi2].
+    + destruct (IHT1 i Hlin1 Hi1) as (Π₁ & HΠ1).
+      exists (Π₁++[CtxSemicL (bterm_ctx_act T2 Δs)]).
+      intros Γ. rewrite fill_app /=.
+      rewrite HΠ1. f_equiv.
+      assert (i ∉ term_fv T2).
+      { set_solver. }
+      apply bterm_ctx_act_fv.
+      intros j. destruct (decide (i = j)) as [->|?].
+      { naive_solver. }
+      rewrite functions.fn_lookup_insert_ne//.
+    + destruct (IHT2 i Hlin2 Hi2) as (Π₁ & HΠ1).
+      exists (Π₁++[CtxSemicR (bterm_ctx_act T1 Δs)]).
+      intros Γ. rewrite fill_app /=.
+      rewrite HΠ1. f_equiv.
+      assert (i ∉ term_fv T1).
+      { set_solver. }
+      apply bterm_ctx_act_fv.
+      intros j. destruct (decide (i = j)) as [->|?].
+      { naive_solver. }
+      rewrite functions.fn_lookup_insert_ne//.
+Qed.
+
+(** ** linearization properties *)
 Lemma linearize_pre_mono T (idx1 : nat):
   idx1 ≤ fst $ fst $ linearize_pre T idx1.
 Proof.
@@ -248,194 +396,22 @@ Proof.
     set_solver by lia.
 Qed.
 
-(** On interpretations/actions of terms: *)
-
-(* Interpretation of bunched terms only depend on free variables *)
-Lemma bterm_ctx_act_fv `{!EqDecision V,!Countable V} (T : bterm V) Δs Γs :
-  (∀ i : V, i ∈ term_fv T → Δs i = Γs i) →
-  bterm_ctx_act T Δs = bterm_ctx_act T Γs.
-Proof.
-  induction T; simpl.
-  - set_solver.
-  - set_unfold. intros H.
-    rewrite IHT1; eauto. rewrite IHT2; eauto.
-  - set_unfold. intros H.
-    rewrite IHT1; eauto. rewrite IHT2; eauto.
-Qed.
-Lemma bterm_alg_act_fv `{!EqDecision V,!Countable V} {PROP : bi}
-      (T : bterm V) Δs Γs :
-  (∀ i : V, i ∈ term_fv T → Δs i ≡ Γs i) →
-  bterm_alg_act T Δs ≡ bterm_alg_act (PROP:=PROP) T Γs.
-Proof.
-  induction T; simpl.
-  - set_solver.
-  - set_unfold. intros H.
-    rewrite IHT1; eauto. rewrite IHT2; eauto.
-  - set_unfold. intros H.
-    rewrite IHT1; eauto. rewrite IHT2; eauto.
-Qed.
-
-Lemma bterm_alg_act_mono {PROP : bi} `{!EqDecision V, !Countable V}
-      (T : bterm V) Xs Ys :
-  (∀ i, Xs i ⊢ Ys i) →
-  bterm_alg_act T Xs ⊢ bterm_alg_act (PROP:=PROP) T Ys.
-Proof.
-  intros HXY. induction T; simpl; auto.
-  all: by rewrite IHT1 IHT2.
-Qed.
-
-Lemma bterm_alg_act_mono' {PROP : bi} `{!EqDecision V, !Countable V}
-      (T : bterm V) Xs Ys :
-  (∀ i, i ∈ term_fv T → Xs i ⊢ Ys i) →
-  bterm_alg_act T Xs ⊢ bterm_alg_act (PROP:=PROP) T Ys.
-Proof.
-  intros HXY. induction T; simpl; eauto.
-  - apply HXY. set_solver.
-  - f_equiv.
-    + apply IHT1. set_solver.
-    + apply IHT2. set_solver.
-  - f_equiv.
-    + apply IHT1. set_solver.
-    + apply IHT2. set_solver.
-Qed.
-
-(***************************************************)
-(** TODO: move this out *)
-(** Code by Blaisorblade  *)
-From stdpp Require Import finite functions.
-Class FiniteDomain {A B M} `{Lookup A B (M B)} (m : M B) := {
-  enum_domain : list A;
-  finite_mapping (a : A) (b : B) :
-    m !! a = Some b -> a ∈ enum_domain;
-}.
-Arguments enum_domain {A B M _} m {_} : assert.
-Section fin_domain.
-  Context `{EqDecision B}.
-  Context {A M} (m : M B) `{FiniteDomain A B M m}.
-  Definition preimage (b : B) : list A :=
-    filter (λ a, m !! a = Some b) (enum_domain m).
-  Context `{!EqDecision A, !Countable A}.
-  Definition preimage_set (b : B) : gset A := list_to_set (preimage b).
-
-  Lemma preimage_eq_1 a b :
-    b ∈ preimage a → m !! b = Some a.
-  Proof. rewrite /preimage elem_of_list_filter. naive_solver. Qed.
-
-  Lemma preimage_eq_2 a b :
-    m !! b = Some a → b ∈ preimage a.
-  Proof.
-    rewrite /preimage elem_of_list_filter. intros ?; split; auto.
-    by eapply finite_mapping.
-  Qed.
-
-  Lemma preimage_eq a b :
-    b ∈ preimage a ↔ m !! b = Some a.
-  Proof. split; [ apply preimage_eq_1 | apply preimage_eq_2 ]. Qed.
-
-  Lemma preimage_set_eq a b :
-    b ∈ preimage_set a ↔ m !! b = Some a.
-  Proof.
-    rewrite /preimage_set elem_of_list_to_set.
-    apply preimage_eq.
-  Qed.
-End fin_domain.
-
-Section finite_preimage.
-  Context `{!EqDecision A, !Finite A} {B : Type} (f : A -> B).
-  #[local] Set Default Proof Using "Type*".
-
-  (* Instance fn_lookup_total : LookupTotal A B (A -> B) := λ a f, f a. *)
-  Instance fn_lookup : Lookup A B (A -> B) := λ a f, Some (f a).
-  #[refine] Global Instance finite_finitedomain : FiniteDomain (M := λ B, A -> B) f :=
-  { enum_domain := enum _ }.
-  Proof. intros; apply elem_of_enum. Defined.
-End finite_preimage.
-
-Section map_preimage.
-  Context {K A : Type} `{FinMap K M}.
-  Context `{!EqDecision A, !Countable A, !EqDecision K, !Countable K}.
-  Variable (m : M A).
-
-  #[refine] Global Instance finmapmap_finitedomain : FiniteDomain m :=
-  { enum_domain := fst <$> map_to_list m }.
-  (* XXX fix set_solver. *)
-  Proof. move=> k a /elem_of_map_to_list. apply: elem_of_list_fmap_1. Defined.
-
-End map_preimage.
-
-Section preimage_properties.
-  Context `{!EqDecision A, !Countable A, !EqDecision K, !Countable K}.
-
-  Lemma preimage_set_singleton i x : preimage_set ({[ i := x ]} : gmap K A) x ≡ {[i]}.
-  Proof.
-    intros z. rewrite preimage_set_eq.
-    rewrite lookup_singleton_Some. set_solver.
-  Qed.
-
-End preimage_properties.
-(** / END TODO *)
-
-Definition list_ap {A B} (fs : list (A → B)) (xs : list A) : list B :=
-  f ← fs;
-  x ← xs;
-  [f x].
-
-Section gset_ap.
-  Context {A B C : Type}.
-  Context `{!EqDecision A, !Countable A, !EqDecision B, !Countable B}.
-  Context `{!EqDecision C, !Countable C}.
-
-  Definition set_map_2 (f : A → B → C) (X : gset A) (Y : gset B) : gset C :=
-    list_to_set (list_ap (map f (elements X)) (elements Y)).
-  Typeclasses Opaque set_map_2.
-
-  Lemma elem_of_map_2 (f : A → B → C) (X : gset A) (Y : gset B) z :
-    z ∈ set_map_2 f X Y ↔ ∃ x y, z = f x y ∧ x ∈ X ∧ y ∈ Y.
-  Proof.
-    unfold set_map_2. rewrite elem_of_list_to_set.
-    rewrite /list_ap. rewrite list_fmap_bind.
-    rewrite elem_of_list_bind. set_solver.
-  Qed.
-  (* Global Instance set_unfold_map (f : A → B) (X : C) (P : A → Prop) y : *)
-  (*   (∀ x, SetUnfoldElemOf x X (P x)) → *)
-  (*   SetUnfoldElemOf y (set_map (D:=D) f X) (∃ x, y = f x ∧ P x). *)
-  (* Proof. constructor. rewrite elem_of_map; naive_solver. Qed. *)
-
-
-End gset_ap.
-
-Global Instance: Params (@set_map_2) 12 := {}.
-
-Fixpoint bterm_gset_fold (T : bterm (gset nat)) : gset (bterm nat) :=
-  match T with
-  | Var X => set_map Var X
-  | TComma T1 T2 =>
-      let S1 := bterm_gset_fold T1 in
-      let S2 := bterm_gset_fold T2 in
-      set_map_2 TComma S1 S2
-  | TSemic T1 T2 =>
-      let S1 := bterm_gset_fold T1 in
-      let S2 := bterm_gset_fold T2 in
-      set_map_2 TSemic S1 S2
-  end.
-
-Definition bterm_gset_fmap (f : nat → nat) (T : bterm (gset nat)) : bterm (gset nat) :=
-  (λ X, set_map f X) <$> T.
+(** ** term folding properties *)
 Lemma bterm_gset_fold_fmap (f : nat → nat) (T : bterm (gset nat)) (T' : bterm nat) :
-  T' ∈ bterm_gset_fold T → (f <$> T') ∈ (bterm_gset_fold (bterm_gset_fmap f T)).
+  T' ∈ bterm_gset_fold T → f <$> T' ∈ (bterm_gset_fold (bterm_gset_fmap f T)).
 Proof.
   revert T'; induction T as [X|T1 HT1 T2 HT2|T1 HT1 T2 HT2]=> T' /=.
   - rewrite elem_of_map.
     intros [x [-> Hx]]. simpl.
     rewrite elem_of_map. exists (f x).
     rewrite elem_of_map. eauto.
-  - rewrite elem_of_map_2.
+  - rewrite sets.elem_of_map_2.
     intros (T1' & T2' & -> & HT1' & HT2').
-    apply elem_of_map_2. exists (f <$> T1'),(f <$> T2').
+    apply sets.elem_of_map_2. exists (f <$> T1'),(f <$> T2').
     naive_solver.
-  - rewrite elem_of_map_2.
+  - rewrite sets.elem_of_map_2.
     intros (T1' & T2' & -> & HT1' & HT2').
-    apply elem_of_map_2. exists (f <$> T1'),(f <$> T2').
+    apply sets.elem_of_map_2. exists (f <$> T1'),(f <$> T2').
     naive_solver.
 Qed.
 Lemma bterm_gset_fold_fmap_inv (f : nat → gset nat) (T T' : bterm nat) :
@@ -445,7 +421,7 @@ Proof.
   revert T'. induction T as [x|T1 HT1 T2 HT2|T1 HT1 T2 HT2]=> T' Hlin /=.
   - rewrite elem_of_map. intros [y [-> Hy]]. exists (const y). split; eauto.
     intros i. simpl. rewrite elem_of_singleton. naive_solver.
-  - rewrite elem_of_map_2.
+  - rewrite sets.elem_of_map_2.
     intros (T1' & T2' & -> & HT1' & HT2').
     destruct Hlin as [Hfv [Hlin1 Hlin2]].
     destruct (HT1 _ Hlin1 HT1') as [g1 [Hg1 Hg1']].
@@ -465,7 +441,7 @@ Proof.
       apply bterm_fmap_ext; auto.
       intros x Hx. assert (x ∉ term_fv T1) by set_solver.
       rewrite decide_False //. }
-  - rewrite elem_of_map_2.
+  - rewrite sets.elem_of_map_2.
     intros (T1' & T2' & -> & HT1' & HT2').
     destruct Hlin as [Hfv [Hlin1 Hlin2]].
     destruct (HT1 _ Hlin1 HT1') as [g1 [Hg1 Hg1']].
@@ -487,539 +463,7 @@ Proof.
       rewrite decide_False //. }
 Qed.
 
-Section linearize_bterm_properties.
-  Context {PROP : bi}.
-  Variable (T : bterm nat).
-  Implicit Type Xs Ys : nat → PROP.
-  Implicit Type n k m : nat.
 
-  Definition linearize_bterm_ren_act Xs : nat → PROP :=
-    λ (n : nat), Xs (linearize_bterm_ren T !!! n).
-
-  Definition ren_inverse : nat → gset nat := preimage_set (linearize_bterm_ren T).
-  Definition disj_ren_inverse Xs : nat → PROP := λ n, (∃ k, ⌜k ∈ ren_inverse n⌝ ∧ Xs k)%I.
-
-  Definition transform_premise (Tz : bterm nat) : gset (bterm nat).
-  Proof.
-    refine (let Tn' := linearize_bterm Tz in _).
-    refine (let T'' := bterm_fmap _ _ (λ j, ren_inverse (linearize_bterm_ren Tz !!! j)) Tn' in _).
-    apply (bterm_gset_fold T'').
-  Defined.
-
-  Lemma linearize_bterm_act Xs :
-    bterm_alg_act (linearize_bterm T) Xs ⊢ bterm_alg_act T (disj_ren_inverse Xs).
-  Proof.
-    rewrite /disj_ren_inverse /ren_inverse /linearize_bterm_ren /linearize_bterm.
-    generalize 0.
-    induction T as [x | T1 IHT1 T2 IHT2 | T1 IHT1 T2 IHT2 ]=>i; simpl.
-    - apply (bi.exist_intro' _ _ i).
-      rewrite preimage_set_singleton.
-      apply bi.and_intro; eauto. apply bi.pure_intro. set_solver.
-    - specialize (IHT1 i).
-      destruct (linearize_pre T1 i) as [[i1 m1] T1'] eqn:Ht1.
-      specialize (IHT2 i1).
-      destruct (linearize_pre T2 i1) as [[i2 m2] T2'] eqn:Ht2. simpl.
-      assert (dom (gset _) m1 = set_seq i (i1-i)) as Hm1.
-      { replace i1 with (fst $ fst (linearize_pre T1 i)) by rewrite Ht1 //.
-        replace m1 with (snd $ fst (linearize_pre T1 i)) by rewrite Ht1 //.
-        apply linearize_pre_dom. }
-      assert (dom (gset _) m2 = set_seq i1 (i2-i1)) as Hm2.
-      { replace i2 with (fst $ fst (linearize_pre T2 i1)) by rewrite Ht2 //.
-        replace m2 with (snd $ fst (linearize_pre T2 i1)) by rewrite Ht2 //.
-        apply linearize_pre_dom. }
-      assert (m1 ##ₘ m2) as Hm1m2disj.
-      { apply map_disjoint_dom_2. rewrite Hm1 Hm2.
-        set_unfold. lia. }
-      f_equiv.
-      { rewrite IHT1 /=.
-        apply bterm_alg_act_mono=>j.
-        apply bi.exist_mono'=>k. do 2 f_equiv.
-        rewrite !preimage_set_eq. intro. by apply lookup_union_Some_l. }
-      { rewrite IHT2 /=.
-        apply bterm_alg_act_mono=>j.
-        apply bi.exist_mono'=>k. do 2 f_equiv.
-        rewrite !preimage_set_eq. intro. by apply lookup_union_Some_r. }
-    - specialize (IHT1 i).
-      destruct (linearize_pre T1 i) as [[i1 m1] T1'] eqn:Ht1.
-      specialize (IHT2 i1).
-      destruct (linearize_pre T2 i1) as [[i2 m2] T2'] eqn:Ht2. simpl.
-      assert (dom (gset _) m1 = set_seq i (i1-i)) as Hm1.
-      { replace i1 with (fst $ fst (linearize_pre T1 i)) by rewrite Ht1 //.
-        replace m1 with (snd $ fst (linearize_pre T1 i)) by rewrite Ht1 //.
-        apply linearize_pre_dom. }
-      assert (dom (gset _) m2 = set_seq i1 (i2-i1)) as Hm2.
-      { replace i2 with (fst $ fst (linearize_pre T2 i1)) by rewrite Ht2 //.
-        replace m2 with (snd $ fst (linearize_pre T2 i1)) by rewrite Ht2 //.
-        apply linearize_pre_dom. }
-      assert (m1 ##ₘ m2) as Hm1m2disj.
-      { apply map_disjoint_dom_2. rewrite Hm1 Hm2.
-        set_unfold. lia. }
-      f_equiv.
-      { rewrite IHT1 /=.
-        apply bterm_alg_act_mono=>j.
-        apply bi.exist_mono'=>k. do 2 f_equiv.
-        rewrite !preimage_set_eq. intro. by apply lookup_union_Some_l. }
-      { rewrite IHT2 /=.
-        apply bterm_alg_act_mono=>j.
-        apply bi.exist_mono'=>k. do 2 f_equiv.
-        rewrite !preimage_set_eq. intro. by apply lookup_union_Some_r. }
-  Qed.
-
-  Lemma bterm_alg_act_renaming'' Tz Xs :
-    bterm_alg_act Tz (linearize_bterm_ren_act Xs) ≡ bterm_alg_act ((λ n, linearize_bterm_ren T !!! n) <$> Tz) Xs.
-  Proof.
-    rewrite /linearize_bterm_ren_act.
-    induction Tz as [x | T1 IHT1 T2 IHT2 | T1 IHT1 T2 IHT2 ]; eauto; simpl; by f_equiv.
-  Qed.
-
-  Lemma ren_ren_inverse i j :
-    j ∈ ren_inverse i → linearize_bterm_ren T !!! j = i.
-  Proof.
-    rewrite /ren_inverse. rewrite preimage_set_eq.
-    apply lookup_total_correct.
-  Qed.
-  (* Lemma ren_inverse_ren i j : *)
-  (*   linearize_bterm_ren T !!! j = i → j ∈ ren_inverse i. *)
-  (* Proof. *)
-  (*   rewrite /ren_inverse. rewrite preimage_set_eq. *)
-  (*   intros <-. apply lookup_lookup_total. *)
-  (* Qed. *)
-
-  (* TODO: move *)
-  Local Lemma pure_left_absorb (φ : Prop) (Q : PROP) :
-      (⌜ φ ⌝ ∗ Q) ⊢ ⌜ φ ⌝.
-  Proof.
-    apply bi.wand_elim_l'. apply bi.pure_elim'=>Hϕ.
-    apply bi.wand_intro_l. by apply bi.pure_intro.
-  Qed.
-
-  Lemma bterm_alg_act_disj_ren_inverse_transform Tz Xs :
-    bterm_alg_act Tz (disj_ren_inverse Xs) -∗ ∃ Tk, ⌜Tk ∈ transform_premise Tz⌝ ∧ bterm_alg_act Tk Xs.
-  Proof.
-    rewrite /disj_ren_inverse /transform_premise /linearize_bterm /linearize_bterm_ren.
-    generalize 0.
-    induction Tz as [x | T1 IHT1 T2 IHT2 | T1 IHT1 T2 IHT2 ]=>idx; simpl.
-    - apply bi.exist_elim=>k. apply bi.pure_elim_l=>Hk.
-      apply (bi.exist_intro' _ _ (Var k)). apply bi.and_intro; eauto.
-      apply bi.pure_intro.
-      eapply fin_sets.elem_of_map_2. by rewrite lookup_total_singleton.
-    - specialize (IHT1 idx).
-      destruct (linearize_pre T1 idx) as [[idx1 m1] T1'] eqn:Ht1.
-      specialize (IHT2 idx1).
-      destruct (linearize_pre T2 idx1) as [[idx2 m2] T2'] eqn:Ht2.
-
-      assert (dom (gset _) m1 = set_seq idx (idx1-idx)) as Hm1.
-      { replace idx1 with (fst $ fst (linearize_pre T1 idx)) by rewrite Ht1 //.
-        replace m1 with (snd $ fst (linearize_pre T1 idx)) by rewrite Ht1 //.
-        apply linearize_pre_dom. }
-      assert (dom (gset _) m2 = set_seq idx1 (idx2-idx1)) as Hm2.
-      { replace idx2 with (fst $ fst (linearize_pre T2 idx1)) by rewrite Ht2 //.
-        replace m2 with (snd $ fst (linearize_pre T2 idx1)) by rewrite Ht2 //.
-        apply linearize_pre_dom. }
-      assert (m1 ##ₘ m2) as Hm1m2disj.
-      { apply map_disjoint_dom_2. rewrite Hm1 Hm2.
-        set_unfold. lia. }
-
-      assert (term_fv T1' ⊆ set_seq idx (idx1-idx)) as Hfv1.
-      { replace T1' with (snd (linearize_pre T1 idx)) by rewrite Ht1 //.
-        replace idx1 with (fst $ fst (linearize_pre T1 idx)) by rewrite Ht1 //.
-        apply linearize_pre_fv. }
-      assert (term_fv T2' ⊆ set_seq idx1 (idx2-idx1)) as Hfv2.
-      { replace T2' with (snd (linearize_pre T2 idx1)) by rewrite Ht2 //.
-        replace idx2 with (fst $ fst (linearize_pre T2 idx1)) by rewrite Ht2 //.
-        apply linearize_pre_fv. }
-
-      rewrite IHT1 . rewrite bi.sep_exist_r. apply bi.exist_elim=>Tk1.
-      rewrite bi.sep_and_r. rewrite pure_left_absorb.
-      apply bi.pure_elim_l=>Hk1.
-      rewrite IHT2. rewrite comm. rewrite bi.sep_exist_r. apply bi.exist_elim=>Tk2.
-      rewrite bi.sep_and_r. rewrite pure_left_absorb.
-      apply bi.pure_elim_l=>Hk2. rewrite comm.
-      apply (bi.exist_intro' _ _ (TComma Tk1 Tk2)). apply bi.and_intro; simpl; last by f_equiv.
-      apply bi.pure_intro.
-      apply elem_of_map_2. eexists _,_. repeat split; eauto.
-      + simpl in Hk1.
-        enough ((λ j : nat, ren_inverse (m1 !!! j)) <$> T1' = ((λ j : nat, ren_inverse ((m1 ∪ m2) !!! j)) <$> T1'))
-          as <-; first done.
-        apply bterm_fmap_ext; last done. intros x Hx. f_equiv.
-        rewrite !lookup_total_alt. f_equiv.
-        symmetry. apply lookup_union_l. apply elem_of_dom.
-        set_unfold. naive_solver.
-      + simpl in Hk2.
-        enough ((λ j : nat, ren_inverse (m2 !!! j)) <$> T2' = ((λ j : nat, ren_inverse ((m1 ∪ m2) !!! j)) <$> T2'))
-          as <-; first done.
-        apply bterm_fmap_ext; last done. intros x Hx. f_equiv.
-        rewrite !lookup_total_alt. f_equiv.
-        symmetry. apply lookup_union_r. apply not_elem_of_dom.
-        set_unfold. intros Hx'. apply Hfv2 in Hx. apply Hm1 in Hx'. lia.
-    - specialize (IHT1 idx).
-      destruct (linearize_pre T1 idx) as [[idx1 m1] T1'] eqn:Ht1.
-      specialize (IHT2 idx1).
-      destruct (linearize_pre T2 idx1) as [[idx2 m2] T2'] eqn:Ht2.
-
-      assert (dom (gset _) m1 = set_seq idx (idx1-idx)) as Hm1.
-      { replace idx1 with (fst $ fst (linearize_pre T1 idx)) by rewrite Ht1 //.
-        replace m1 with (snd $ fst (linearize_pre T1 idx)) by rewrite Ht1 //.
-        apply linearize_pre_dom. }
-      assert (dom (gset _) m2 = set_seq idx1 (idx2-idx1)) as Hm2.
-      { replace idx2 with (fst $ fst (linearize_pre T2 idx1)) by rewrite Ht2 //.
-        replace m2 with (snd $ fst (linearize_pre T2 idx1)) by rewrite Ht2 //.
-        apply linearize_pre_dom. }
-      assert (m1 ##ₘ m2) as Hm1m2disj.
-      { apply map_disjoint_dom_2. rewrite Hm1 Hm2.
-        set_unfold. lia. }
-
-      assert (term_fv T1' ⊆ set_seq idx (idx1-idx)) as Hfv1.
-      { replace T1' with (snd (linearize_pre T1 idx)) by rewrite Ht1 //.
-        replace idx1 with (fst $ fst (linearize_pre T1 idx)) by rewrite Ht1 //.
-        apply linearize_pre_fv. }
-      assert (term_fv T2' ⊆ set_seq idx1 (idx2-idx1)) as Hfv2.
-      { replace T2' with (snd (linearize_pre T2 idx1)) by rewrite Ht2 //.
-        replace idx2 with (fst $ fst (linearize_pre T2 idx1)) by rewrite Ht2 //.
-        apply linearize_pre_fv. }
-
-      rewrite IHT1. rewrite bi.and_exist_r. apply bi.exist_elim=>Tk1.
-      rewrite -assoc.
-      apply bi.pure_elim_l=>Hk1.
-      rewrite IHT2. rewrite comm. rewrite bi.and_exist_r. apply bi.exist_elim=>Tk2.
-      rewrite -assoc.
-      apply bi.pure_elim_l=>Hk2. rewrite comm.
-      apply (bi.exist_intro' _ _ (TSemic Tk1 Tk2)). apply bi.and_intro; simpl; last by f_equiv.
-      apply bi.pure_intro.
-      apply elem_of_map_2. eexists _,_. repeat split; eauto.
-      + simpl in Hk1.
-        enough ((λ j : nat, ren_inverse (m1 !!! j)) <$> T1' = ((λ j : nat, ren_inverse ((m1 ∪ m2) !!! j)) <$> T1'))
-          as <-; first done.
-        apply bterm_fmap_ext; last done. intros x Hx. f_equiv.
-        rewrite !lookup_total_alt. f_equiv.
-        symmetry. apply lookup_union_l. apply elem_of_dom.
-        set_unfold. naive_solver.
-      + simpl in Hk2.
-        enough ((λ j : nat, ren_inverse (m2 !!! j)) <$> T2' = ((λ j : nat, ren_inverse ((m1 ∪ m2) !!! j)) <$> T2'))
-          as <-; first done.
-        apply bterm_fmap_ext; last done. intros x Hx. f_equiv.
-        rewrite !lookup_total_alt. f_equiv.
-        symmetry. apply lookup_union_r. apply not_elem_of_dom.
-        set_unfold. intros Hx'. apply Hfv2 in Hx. apply Hm1 in Hx'. lia.
-  Qed.
-
-  Lemma elem_of_map_ren_ren_inverse x y :
-    y ∈ (set_map (C:=gset nat) (λ n, linearize_bterm_ren T !!! n) (ren_inverse x) : gset nat) → y = x.
-  Proof.
-    rewrite elem_of_map.
-    intros [z [-> Hz]]. by apply ren_ren_inverse.
-  Qed.
-
-  Lemma transformed_premise_act_ren Tz' Tz Xs :
-    Tz' ∈ transform_premise Tz → bterm_alg_act Tz' (linearize_bterm_ren_act Xs) ≡ bterm_alg_act Tz Xs.
-  Proof.
-    rewrite /transform_premise.
-    intros H1.
-    apply (bterm_gset_fold_fmap (λ n, linearize_bterm_ren T !!! n)) in H1.
-    revert H1.
-    rewrite /bterm_gset_fmap.
-    rewrite -(bterm_fmap_compose (λ j : nat, ren_inverse (linearize_bterm_ren Tz !!! j))).
-    rewrite bterm_alg_act_renaming''.
-    intros H1. f_equiv.
-    revert H1.
-    pose (Tz'' := (λ n, linearize_bterm_ren T !!! n) <$> Tz').
-    fold Tz''. intros HTz''.
-    assert (Tz'' ∈ bterm_gset_fold
-                ((λ j : nat, set_map (λ n, linearize_bterm_ren T !!! n) (ren_inverse (linearize_bterm_ren Tz !!! j))) <$> linearize_bterm Tz)) as HH.
-    {  apply HTz''. }
-    clear HTz''.
-    apply bterm_gset_fold_fmap_inv in HH; last first.
-    { apply linearize_pre_linear. }
-    destruct HH as [g [Hg ->]].
-    assert (∀ i : nat,
-           i ∈ term_fv (linearize_bterm Tz)
-         → g i = (linearize_bterm_ren Tz !!! i)) as HHH.
-    { intros i Hi. apply elem_of_map_ren_ren_inverse.
-      by eapply Hg. }
-    clear Hg. revert HHH.
-    rewrite /(linearize_bterm_ren Tz) /(linearize_bterm Tz).
-    generalize 0.
-    induction Tz as [x | T1 IHT1 T2 IHT2 | T1 IHT1 T2 IHT2 ]=>i; simpl.
-    - intros H1. f_equiv.
-      etrans. { apply H1. by apply elem_of_singleton. }
-      apply lookup_total_singleton.
-    - intros H1.
-      specialize (IHT1 i).
-      destruct (linearize_pre T1 i) as [[i1 m1] T1'] eqn:Ht1.
-      specialize (IHT2 i1).
-      destruct (linearize_pre T2 i1) as [[i2 m2] T2'] eqn:Ht2.
-      assert (term_fv T1' ⊆ set_seq i (i1-i)).
-      { replace T1' with (snd (linearize_pre T1 i)) by rewrite Ht1 //.
-        replace i1 with (fst $ fst (linearize_pre T1 i)) by rewrite Ht1 //.
-        apply linearize_pre_fv. }
-      assert (term_fv T2' ⊆ set_seq i1 (i2-i1)).
-      { replace T2' with (snd (linearize_pre T2 i1)) by rewrite Ht2 //.
-        replace i2 with (fst $ fst (linearize_pre T2 i1)) by rewrite Ht2 //.
-        apply linearize_pre_fv. }
-      assert (dom (gset _) m1 = set_seq i (i1-i)) as Hm1.
-      { replace i1 with (fst $ fst (linearize_pre T1 i)) by rewrite Ht1 //.
-        replace m1 with (snd $ fst (linearize_pre T1 i)) by rewrite Ht1 //.
-        apply linearize_pre_dom. }
-      assert (dom (gset _) m2 = set_seq i1 (i2-i1)) as Hm2.
-      { replace i2 with (fst $ fst (linearize_pre T2 i1)) by rewrite Ht2 //.
-        replace m2 with (snd $ fst (linearize_pre T2 i1)) by rewrite Ht2 //.
-        apply linearize_pre_dom. }
-      simpl. f_equiv.
-      { apply IHT1. intros j Hj. simpl in *. trans ((m1 ∪ m2) !!! j).
-        - apply H1. set_solver.
-        - rewrite !lookup_total_alt. f_equiv.
-          apply lookup_union_l.
-          apply elem_of_dom. rewrite Hm1. naive_solver. }
-      { apply IHT2. intros j Hj. simpl in *. trans ((m1 ∪ m2) !!! j).
-        - apply H1. set_solver.
-        - rewrite !lookup_total_alt. f_equiv.
-          apply lookup_union_r. apply not_elem_of_dom.
-          rewrite Hm1. set_unfold. naive_solver lia. }
-    - intros H1.
-      specialize (IHT1 i).
-      destruct (linearize_pre T1 i) as [[i1 m1] T1'] eqn:Ht1.
-      specialize (IHT2 i1).
-      destruct (linearize_pre T2 i1) as [[i2 m2] T2'] eqn:Ht2.
-      assert (term_fv T1' ⊆ set_seq i (i1-i)).
-      { replace T1' with (snd (linearize_pre T1 i)) by rewrite Ht1 //.
-        replace i1 with (fst $ fst (linearize_pre T1 i)) by rewrite Ht1 //.
-        apply linearize_pre_fv. }
-      assert (term_fv T2' ⊆ set_seq i1 (i2-i1)).
-      { replace T2' with (snd (linearize_pre T2 i1)) by rewrite Ht2 //.
-        replace i2 with (fst $ fst (linearize_pre T2 i1)) by rewrite Ht2 //.
-        apply linearize_pre_fv. }
-      assert (dom (gset _) m1 = set_seq i (i1-i)) as Hm1.
-      { replace i1 with (fst $ fst (linearize_pre T1 i)) by rewrite Ht1 //.
-        replace m1 with (snd $ fst (linearize_pre T1 i)) by rewrite Ht1 //.
-        apply linearize_pre_dom. }
-      assert (dom (gset _) m2 = set_seq i1 (i2-i1)) as Hm2.
-      { replace i2 with (fst $ fst (linearize_pre T2 i1)) by rewrite Ht2 //.
-        replace m2 with (snd $ fst (linearize_pre T2 i1)) by rewrite Ht2 //.
-        apply linearize_pre_dom. }
-      simpl. f_equiv.
-      { apply IHT1. intros j Hj. simpl in *. trans ((m1 ∪ m2) !!! j).
-        - apply H1. set_solver.
-        - rewrite !lookup_total_alt. f_equiv.
-          apply lookup_union_l.
-          apply elem_of_dom. rewrite Hm1. naive_solver. }
-      { apply IHT2. intros j Hj. simpl in *. trans ((m1 ∪ m2) !!! j).
-        - apply H1. set_solver.
-        - rewrite !lookup_total_alt. f_equiv.
-          apply lookup_union_r. apply not_elem_of_dom.
-          rewrite Hm1. set_unfold. naive_solver lia. }
-  Qed.
-
-  Lemma linearize_bterm_act_ren Xs:
-    bterm_alg_act (linearize_bterm T) (linearize_bterm_ren_act Xs) ≡ bterm_alg_act T Xs.
-  Proof.
-    rewrite /linearize_bterm_ren_act /linearize_bterm_ren /linearize_bterm.
-    generalize 0.
-    induction T as [x | T1 IHT1 T2 IHT2 | T1 IHT1 T2 IHT2 ]=>i; simpl.
-    - by rewrite lookup_total_singleton.
-    - specialize (IHT1 i).
-      destruct (linearize_pre T1 i) as [[i1 m1] T1'] eqn:Ht1.
-      specialize (IHT2 i1).
-      destruct (linearize_pre T2 i1) as [[i2 m2] T2'] eqn:Ht2.
-      assert (term_fv T1' ⊆ set_seq i (i1-i)).
-      { replace T1' with (snd (linearize_pre T1 i)) by rewrite Ht1 //.
-        replace i1 with (fst $ fst (linearize_pre T1 i)) by rewrite Ht1 //.
-        apply linearize_pre_fv. }
-      assert (term_fv T2' ⊆ set_seq i1 (i2-i1)).
-      { replace T2' with (snd (linearize_pre T2 i1)) by rewrite Ht2 //.
-        replace i2 with (fst $ fst (linearize_pre T2 i1)) by rewrite Ht2 //.
-        apply linearize_pre_fv. }
-      assert (dom (gset _) m1 = set_seq i (i1-i)) as Hm1.
-      { replace i1 with (fst $ fst (linearize_pre T1 i)) by rewrite Ht1 //.
-        replace m1 with (snd $ fst (linearize_pre T1 i)) by rewrite Ht1 //.
-        apply linearize_pre_dom. }
-      assert (dom (gset _) m2 = set_seq i1 (i2-i1)) as Hm2.
-      { replace i2 with (fst $ fst (linearize_pre T2 i1)) by rewrite Ht2 //.
-        replace m2 with (snd $ fst (linearize_pre T2 i1)) by rewrite Ht2 //.
-        apply linearize_pre_dom. }
-      simpl. repeat split; eauto.
-      rewrite -IHT1 -IHT2. f_equiv.
-      + eapply bterm_alg_act_fv.
-        intros j Hj.
-        assert ((m1 ∪ m2) !!! j = m1 !!! j) as ->; eauto.
-        unfold lookup_total, map_lookup_total. f_equiv.
-        apply lookup_union_l, elem_of_dom. rewrite Hm1. set_solver by lia.
-      + eapply bterm_alg_act_fv.
-        intros j Hj.
-        assert ((m1 ∪ m2) !!! j = m2 !!! j) as ->; eauto.
-        unfold lookup_total, map_lookup_total. f_equiv.
-        apply lookup_union_r. apply not_elem_of_dom. rewrite Hm1. set_solver by lia.
-    - specialize (IHT1 i).
-      destruct (linearize_pre T1 i) as [[i1 m1] T1'] eqn:Ht1.
-      specialize (IHT2 i1).
-      destruct (linearize_pre T2 i1) as [[i2 m2] T2'] eqn:Ht2.
-      assert (term_fv T1' ⊆ set_seq i (i1-i)).
-      { replace T1' with (snd (linearize_pre T1 i)) by rewrite Ht1 //.
-        replace i1 with (fst $ fst (linearize_pre T1 i)) by rewrite Ht1 //.
-        apply linearize_pre_fv. }
-      assert (term_fv T2' ⊆ set_seq i1 (i2-i1)).
-      { replace T2' with (snd (linearize_pre T2 i1)) by rewrite Ht2 //.
-        replace i2 with (fst $ fst (linearize_pre T2 i1)) by rewrite Ht2 //.
-        apply linearize_pre_fv. }
-      assert (dom (gset _) m1 = set_seq i (i1-i)) as Hm1.
-      { replace i1 with (fst $ fst (linearize_pre T1 i)) by rewrite Ht1 //.
-        replace m1 with (snd $ fst (linearize_pre T1 i)) by rewrite Ht1 //.
-        apply linearize_pre_dom. }
-      assert (dom (gset _) m2 = set_seq i1 (i2-i1)) as Hm2.
-      { replace i2 with (fst $ fst (linearize_pre T2 i1)) by rewrite Ht2 //.
-        replace m2 with (snd $ fst (linearize_pre T2 i1)) by rewrite Ht2 //.
-        apply linearize_pre_dom. }
-      simpl. repeat split; eauto.
-      rewrite -IHT1 -IHT2. f_equiv.
-      + eapply bterm_alg_act_fv.
-        intros j Hj.
-        assert ((m1 ∪ m2) !!! j = m1 !!! j) as ->; eauto.
-        unfold lookup_total, map_lookup_total. f_equiv.
-        apply lookup_union_l, elem_of_dom. rewrite Hm1. set_solver by lia.
-      + eapply bterm_alg_act_fv.
-        intros j Hj.
-        assert ((m1 ∪ m2) !!! j = m2 !!! j) as ->; eauto.
-        unfold lookup_total, map_lookup_total. f_equiv.
-        apply lookup_union_r. apply not_elem_of_dom. rewrite Hm1. set_solver by lia.
-  Qed.
-
-End linearize_bterm_properties.
-
-
-(* Definition t0 := (TSemic (TComma (Var 1) (Var 1)) (Var 2)). *)
-(* Definition t1 := (TSemic (TComma (Var 1) (Var 2)) (Var 2)). *)
-(* Eval compute in (linearize_bterm t0). *)
-(* Eval vm_compute in (elements $ ren_inverse t0 0). *)
-(* Eval vm_compute in (elements $ transform_premise t0 t1). *)
-
-Definition structural_rule := (list (bterm nat) * bterm nat)%type.
-
-Definition analytic_completion (s : structural_rule) : structural_rule :=
-  let '(Ts,T) := s in
-  (mjoin $ fmap (elements ∘ (transform_premise T)) Ts, linearize_bterm T).
-
-(* restricted form of weakening: [a ∗ a ≤ a]
-   and it's analytic presentation [a₁ * a₂ ≤ a₁ ∨ a₂] *)
-Definition rule_restr_weakn : structural_rule := ([Var 0], TComma (Var 0) (Var 0)).
-Definition rule_restr_weakn_a := analytic_completion rule_restr_weakn.
-Eval vm_compute in rule_restr_weakn_a.
-
-Definition rule_valid (s : structural_rule) (PROP : bi) : Prop :=
-  let '(Ts, T) := s in
-  ∀ (Xs : nat → PROP),
-    bterm_alg_act T Xs ⊢
-       ∃ Ti' : {Ti : bterm nat | Ti ∈ Ts }, bterm_alg_act (proj1_sig Ti') Xs.
-
-Lemma analytic_completion_valid (s : structural_rule) (PROP : bi) :
-  rule_valid (analytic_completion s) PROP → rule_valid s PROP.
-Proof.
-  destruct s as [Ts T].
-  rewrite /rule_valid /=. intros H1 Xs.
-  rewrite -linearize_bterm_act_ren.
-  rewrite H1. apply bi.exist_elim=>Ti.
-  destruct Ti as [Ti HTi]. simpl.
-  apply elem_of_list_join in HTi.
-  destruct HTi as [L [HTi HL]].
-  apply elem_of_list_fmap_2 in HL.
-  destruct HL as [Tz [-> HTz]].
-  apply (bi.exist_intro' _ _  (Tz ↾ HTz)).
-  simpl in *. apply elem_of_elements in HTi.
-  eapply transformed_premise_act_ren in HTi.
-  by rewrite HTi.
-Qed.
-
-Lemma analytic_completion_complete (s : structural_rule) (PROP : bi) :
-  rule_valid s PROP → rule_valid (analytic_completion s) PROP.
-Proof.
-  destruct s as [Ts T].
-  rewrite /rule_valid /=. intros H1 Xs.
-  rewrite linearize_bterm_act.
-  rewrite H1. apply bi.exist_elim=>Ti.
-  destruct Ti as [Ti HTi]. simpl.
-  remember (transform_premise T Ti) as Tzs.
-  rewrite bterm_alg_act_disj_ren_inverse_transform.
-  apply bi.exist_elim=>Tk. apply bi.pure_elim_l=>Htk.
-  assert (Tk ∈ mjoin (fmap (elements ∘ transform_premise T) Ts)) as Tk'.
-  { apply elem_of_list_join. exists (elements (transform_premise T Ti)).
-    split.
-    - by apply elem_of_elements.
-    - rewrite list_fmap_compose.
-      by do 2 apply elem_of_list_fmap_1. }
-  apply (bi.exist_intro' _ _  (Tk ↾ Tk')); done.
-Qed.
-
-(** Interpretation of bunches is a homomorphism w.r.t. bunched terms:
-<<
-  ⟦ T(Δs) ⟧ = ⟦ T ⟧ (⟦ Δs ⟧)
->>
-*)
-Lemma bterm_ctx_alg_act {PROP : bi} `{!EqDecision V,!Countable V}
-      (T : bterm V) (Δs : V → bunch) (s : atom → PROP) :
-  bunch_interp s (bterm_ctx_act T Δs) =
-  bterm_alg_act T (bunch_interp s ∘ Δs).
-Proof.
-  induction T; simpl.
-  - reflexivity.
-  - by rewrite IHT1 IHT2.
-  - by rewrite IHT1 IHT2.
-Qed.
-
-(** Linear bunched terms can be viewed as _bunches with holes_, when
-restricted to one free variable. *)
-Lemma blinterm_ctx_act_insert `{!EqDecision V, !Countable V} (T : bterm V) Δs i :
-  linear_bterm T →
-  i ∈ term_fv T →
-  ∃ (Π : bunch_ctx), ∀ Γ , fill Π Γ = bterm_ctx_act T (<[i:=Γ]>Δs).
-Proof.
-  revert i. induction T=>i; simpl ; intros Hlin Hi.
-  - exists []. intros Γ. assert ( i = x) as -> by set_solver.
-    by rewrite functions.fn_lookup_insert.
-  - destruct Hlin as (Hdisj & Hlin1 & Hlin2).
-    set_unfold.
-    destruct Hi as [Hi1 | Hi2].
-    + destruct (IHT1 i Hlin1 Hi1) as (Π₁ & HΠ1).
-      exists (Π₁++[CtxCommaL (bterm_ctx_act T2 Δs)]).
-      intros Γ. rewrite fill_app /=.
-      rewrite HΠ1. f_equiv.
-      assert (i ∉ term_fv T2).
-      { set_solver. }
-      apply bterm_ctx_act_fv.
-      intros j. destruct (decide (i = j)) as [->|?].
-      { naive_solver. }
-      rewrite functions.fn_lookup_insert_ne//.
-    + destruct (IHT2 i Hlin2 Hi2) as (Π₁ & HΠ1).
-      exists (Π₁++[CtxCommaR (bterm_ctx_act T1 Δs)]).
-      intros Γ. rewrite fill_app /=.
-      rewrite HΠ1. f_equiv.
-      assert (i ∉ term_fv T1).
-      { set_solver. }
-      apply bterm_ctx_act_fv.
-      intros j. destruct (decide (i = j)) as [->|?].
-      { naive_solver. }
-      rewrite functions.fn_lookup_insert_ne//.
-  - destruct Hlin as (Hdisj & Hlin1 & Hlin2).
-    set_unfold.
-    destruct Hi as [Hi1 | Hi2].
-    + destruct (IHT1 i Hlin1 Hi1) as (Π₁ & HΠ1).
-      exists (Π₁++[CtxSemicL (bterm_ctx_act T2 Δs)]).
-      intros Γ. rewrite fill_app /=.
-      rewrite HΠ1. f_equiv.
-      assert (i ∉ term_fv T2).
-      { set_solver. }
-      apply bterm_ctx_act_fv.
-      intros j. destruct (decide (i = j)) as [->|?].
-      { naive_solver. }
-      rewrite functions.fn_lookup_insert_ne//.
-    + destruct (IHT2 i Hlin2 Hi2) as (Π₁ & HΠ1).
-      exists (Π₁++[CtxSemicR (bterm_ctx_act T1 Δs)]).
-      intros Γ. rewrite fill_app /=.
-      rewrite HΠ1. f_equiv.
-      assert (i ∉ term_fv T1).
-      { set_solver. }
-      apply bterm_ctx_act_fv.
-      intros j. destruct (decide (i = j)) as [->|?].
-      { naive_solver. }
-      rewrite functions.fn_lookup_insert_ne//.
-Qed.
 
 (* XXX: unset the results of loading Equations *)
 Global Obligation Tactic := idtac.
