theories/prelude/sets.v
@@ -1,0 +1,152 @@
+From stdpp Require Import prelude base gmap fin_sets.
+
+(** * Preimage of a [FinMap] *)
+(* This is copied form the MR [https://gitlab.mpi-sws.org/iris/stdpp/-/merge_requests/382/] *)
+
+(** Given a finite map [m] with keys [K] and values [A], the preimage
+[map_preimage m] gives a finite map with keys [A] and values set [A]. The type
+of [map_preimage] is very generic to support different map and set
+implementations. A possible instance is [MKA:=gmap K A], [MADK:=gmap A (gset K)],
+and [DK:=gset K]. *)
+Definition map_preimage `{FinMapToList K A MKA, Empty MADK,
+    PartialAlter A DK MADK, Empty DK, Singleton K DK, Union DK}
+    (m : MKA) : MADK :=
+  map_fold (λ i, partial_alter (λ mX, Some $ {[ i ]} ∪ default ∅ mX)) ∅ m.
+Typeclasses Opaque map_preimage.
+
+Section preimage.
+  (** We restrict the theory to finite sets with Leibniz equality, which is
+  sufficient for [gset], but not for [boolset] or [propset]. The result of the
+  pre-image is a map of sets. To support general sets, we need setoid equality
+  on sets, and thus setoid equality on maps. *)
+  Context `{FinMap K MK, FinMap A MA, FinSet K DK, !LeibnizEquiv DK}.
+  Local Notation map_preimage :=
+    (map_preimage (K:=K) (A:=A) (MKA:=MK A) (MADK:=MA DK) (DK:=DK)).
+  Implicit Types m : MK A.
+
+  Lemma map_preimage_empty : map_preimage ∅ = ∅.
+  Proof. apply map_fold_empty. Qed.
+  Lemma map_preimage_insert m i x :
+    m !! i = None →
+    map_preimage (<[i:=x]> m) =
+      partial_alter (λ mX, Some ({[ i ]} ∪ default ∅ mX)) x (map_preimage m).
+  Proof.
+    intros Hi. refine (map_fold_insert_L _ _ i x m _ Hi).
+    intros j1 j2 x1 x2 m' ? _ _. destruct (decide (x1 = x2)) as [->|?].
+    - rewrite <-!partial_alter_compose.
+      apply partial_alter_ext; intros ? _; f_equal/=. set_solver.
+    - by apply partial_alter_commute.
+  Qed.
+
+  Lemma lookup_preimage_Some_empty m x :
+    map_preimage m !! x ≠ Some ∅.
+  Proof.
+    induction m as [|i x' m ? IH] using map_ind.
+    { by rewrite map_preimage_empty, lookup_empty. }
+    rewrite map_preimage_insert by done. destruct (decide (x = x')) as [->|].
+    - rewrite lookup_partial_alter. intros [=]. set_solver.
+    - rewrite lookup_partial_alter_ne by done. set_solver.
+  Qed.
+
+  Lemma lookup_preimage_None_1 m x i :
+    map_preimage m !! x = None → m !! i ≠ Some x.
+  Proof.
+    induction m as [|i' x' m ? IH] using map_ind; [by rewrite lookup_empty|].
+    rewrite map_preimage_insert by done. destruct (decide (x = x')) as [->|].
+    - by rewrite lookup_partial_alter.
+    - rewrite lookup_partial_alter_ne, lookup_insert_Some by done. naive_solver.
+  Qed.
+
+  Lemma lookup_preimage_Some_1 m X x i :
+    map_preimage m !! x = Some X →
+    i ∈ X ↔ m !! i = Some x.
+  Proof.
+    revert X. induction m as [|i' x' m ? IH] using map_ind; intros X.
+    { by rewrite map_preimage_empty, lookup_empty. }
+    rewrite map_preimage_insert by done. destruct (decide (x = x')) as [->|].
+    - rewrite lookup_partial_alter. intros [= <-].
+      rewrite elem_of_union, elem_of_singleton, lookup_insert_Some.
+      destruct (map_preimage m !! x') as [X'|] eqn:Hx'; simpl.
+      + rewrite IH by done. naive_solver.
+      + apply (lookup_preimage_None_1 _ _ i) in Hx'. set_solver.
+    - rewrite lookup_partial_alter_ne, lookup_insert_Some by done. naive_solver.
+  Qed.
+
+  Lemma lookup_preimage_None m x :
+    map_preimage m !! x = None ↔ ∀ i, m !! i ≠ Some x.
+  Proof.
+    split; [by eauto using lookup_preimage_None_1|].
+    intros Hm. apply eq_None_not_Some; intros [X ?].
+    destruct (set_choose_L X) as [i ?].
+    { intros ->. by eapply lookup_preimage_Some_empty. }
+    by eapply (Hm i), lookup_preimage_Some_1.
+  Qed.
+
+  Lemma lookup_preimage_Some m x X :
+    map_preimage m !! x = Some X ↔ X ≠ ∅ ∧ ∀ i, i ∈ X ↔ m !! i = Some x.
+  Proof.
+    split.
+    - intros HxX. split; [intros ->; by eapply lookup_preimage_Some_empty|].
+      intros j. by apply lookup_preimage_Some_1.
+    - intros [HXne HX]. destruct (map_preimage m !! x) as [X'|] eqn:HX'.
+      + f_equal; apply set_eq; intros i. rewrite HX.
+        by apply lookup_preimage_Some_1.
+      + apply set_choose_L in HXne as [j ?].
+        apply (lookup_preimage_None_1 _ _ j) in HX'. naive_solver.
+  Qed.
+
+  Lemma map_preimage_singleton i x : map_preimage {[i:=x]} = {[x:={[i]}]}.
+  Proof.
+    apply map_eq. intro y.
+    rewrite <- insert_empty. rewrite map_preimage_insert; [ | apply lookup_empty ].
+    destruct (decide (x = y)) as [->|Hxy].
+    - rewrite lookup_singleton.
+      rewrite map_preimage_empty. rewrite lookup_partial_alter, lookup_empty.
+      simpl. f_equal. apply right_id. apply _.
+    - rewrite lookup_singleton_ne; auto.
+      rewrite lookup_partial_alter_ne; auto.
+      rewrite map_preimage_empty. apply lookup_empty.
+  Qed.
+
+  (** XXX This is not part of the MR.. yet? *)
+  Lemma lookup_total_preimage `{EqDecision DK} m i x :
+    i ∈ (map_preimage m !!! x) ↔ m !! i = Some x.
+  Proof.
+    rewrite lookup_total_alt.
+    destruct (map_preimage m !! x) as [X'|] eqn:Hp; simpl.
+    - by apply lookup_preimage_Some.
+    - apply (lookup_preimage_None_1 _ _ i) in Hp.
+      set_solver.
+  Qed.
+
+End preimage.
+
+(** * [set_map_2] *)
+
+Definition list_ap {A B} (fs : list (A → B)) (xs : list A) : list B :=
+  f ← fs;
+  x ← xs;
+  [f x].
+
+Section gset_ap.
+  Context {A B C : Type}.
+  Context `{!EqDecision A, !Countable A, !EqDecision B, !Countable B}.
+  Context `{!EqDecision C, !Countable C}.
+
+  Definition set_map_2 (f : A → B → C) (X : gset A) (Y : gset B) : gset C :=
+    list_to_set (list_ap (map f (elements X)) (elements Y)).
+  Typeclasses Opaque set_map_2.
+
+  Lemma elem_of_map_2 (f : A → B → C) (X : gset A) (Y : gset B) z :
+    z ∈ set_map_2 f X Y ↔ ∃ x y, z = f x y ∧ x ∈ X ∧ y ∈ Y.
+  Proof.
+    unfold set_map_2. rewrite elem_of_list_to_set.
+    unfold list_ap. rewrite list_fmap_bind.
+    rewrite elem_of_list_bind. set_solver.
+  Qed.
+  (* Global Instance set_unfold_map (f : A → B) (X : C) (P : A → Prop) y : *)
+  (*   (∀ x, SetUnfoldElemOf x X (P x)) → *)
+  (*   SetUnfoldElemOf y (set_map (D:=D) f X) (∃ x, y = f x ∧ P x). *)
+  (* Proof. constructor. rewrite elem_of_map; naive_solver. Qed. *)
+End gset_ap.
+Global Instance: Params (@set_map_2) 12 := {}.
